Fixing the test.

Test/git-issues/git-issue-1604h.dfy
@@ -1,4 +1,4 @@
-// RUN: %dafny /compile:1 "%s" > "%t"
+// RUN: %dafny /compile:3 "%s" > "%t"
 // RUN: %diff "%s.expect" "%t"
 
 ghost const zero := 0
@@ -6,11 +6,11 @@ type GhostNat = x : int | x >= zero
 const S: set<int> := {-1, 0, 1};
 type GhostNatInS = x : int | x in (set j: GhostNat | j in S)
 
-function method FailIfNotGhostNat(i: GhostNat): int {
+function method FailIfNotGhostNatInS(i: GhostNatInS): int {
   if i < 0 then 1/0 else i
 }
 
 method Main() {
-  var s := forall x: GhostNatInS | x in S :: FailIfNotGhostNat(x) == x;
+  var s := forall x: GhostNatInS | x in S :: FailIfNotGhostNatInS(x) == x;
   print s;
 }
